Fixes to CapAsmgen
In order to run the backend, we need to:

 - Require capability instead of vanilla RISC-V files.

 - Resolve namespace clashes in those cases where old common and
   backend files are imported by chained requirements. Ideally
   capability namespaces would always take precedence, but this is not
   a problem here.

 - Relatedly, change type declarations to point to capability
   types (e.g., [capsignature] instead of [signature]). Naming
   conventions are not fully consistent, i.e., some of the new types
   have previously been given unique names, while others share their
   names with the original backend types.

 - Port missing definitions added to AST and absent from CapAST for
   use inside helpers.

 - Sketch missing definitions for typechecking and build purposes,
   marking missing or suspect pieces with FIXME tags, as usual.

 - Comment out those lemmas that do not go through, while fixing their
   statements (we do not care about backend proofs at the moment).

 - Add new secure architecture files to Makefile.

Co-authored-by: Sven Argo <sven.argo@rub.de>

cheririscV/CapConventions1.v
@@ -122,28 +122,32 @@ Definition loc_result (s: capsignature) : rpair mreg :=
   | CTint | CTany32 => One R10
   | CTfloat | CTsingle | CTany64 => One F10
   | CTlong => if Archi.ptr64 then One R10 else Twolong R11 R10
-  | _ => (* FIXME *)
+  | _ => One R10 (* FIXME *)
   end.
 
 (** The result registers have types compatible with that given in the signature. *)
 
-Lemma loc_result_type:
-  forall sig,
-  subtype (proj_sig_res sig) (typ_rpair mreg_type (loc_result sig)) = true.
-Proof.
-  intros. unfold loc_result, mreg_type;
-  destruct (proj_sig_res sig); auto; destruct Archi.ptr64; auto.
-Qed.
+(* FIXME: some of these proofs are good as sanity checks
+   (but only when we have fixed the missing cases in the
+   new definitions). *)
+(* Lemma loc_result_type: *)
+(*   forall sig, *)
+(*   subtype (proj_sig_res sig) (CapAST.typ_rpair CapMachregs.mreg_type (loc_result sig)) = true. *)
+(* Proof. *)
+(*   intros. unfold loc_result, mreg_type; *)
+(*   destruct (proj_sig_res sig); auto; destruct Archi.ptr64; auto. *)
+(* Qed. *)
 
 (** The result locations are caller-save registers *)
 
-Lemma loc_result_caller_save:
-  forall (s: signature),
-  forall_rpair (fun r => is_callee_save r = false) (loc_result s).
-Proof.
-  intros. unfold loc_result, is_callee_save;
-  destruct (proj_sig_res s); simpl; auto; destruct Archi.ptr64; simpl; auto.
-Qed.
+(* FIXME *)
+(* Lemma loc_result_caller_save: *)
+(*   forall (s: signature), *)
+(*   forall_rpair (fun r => is_callee_save r = false) (loc_result s). *)
+(* Proof. *)
+(*   intros. unfold loc_result, is_callee_save; *)
+(*   destruct (proj_sig_res s); simpl; auto; destruct Archi.ptr64; simpl; auto. *)
+(* Qed. *)
 
 (** If the result is in a pair of registers, those registers are distinct and have type [Tint] at least. *)
 
@@ -152,8 +156,8 @@ Lemma loc_result_pair:
   match loc_result sg with
   | One _ => True
   | Twolong r1 r2 =>
-       r1 <> r2 /\ proj_sig_res sg = Tlong
-    /\ subtype Tint (mreg_type r1) = true /\ subtype Tint (mreg_type r2) = true 
+       r1 <> r2 /\ proj_sig_res sg = CTlong
+    /\ subtype CTint (mreg_type r1) = true /\ subtype CTint (mreg_type r2) = true
     /\ Archi.ptr64 = false
   end.
 Proof.
@@ -219,19 +223,19 @@ Definition float_param_regs :=
 Definition float_extra_param_regs :=
   F0 :: F1 :: F2 :: F3 :: F4 :: F5 :: F6 :: F7 :: nil.
 
-Definition int_arg (ri rf ofs: Z) (ty: typ)
-                   (rec: Z -> Z -> Z -> list (rpair loc)) :=
+Definition int_arg (ri rf ofs: Z) (ty: captyp)
+                   (rec: Z -> Z -> Z -> list (rpair caploc)) :=
   match list_nth_z int_param_regs ri with
   | Some r =>
       One(R r) :: rec (ri + 1) rf ofs
   | None   =>
-      let ofs := align ofs (typesize ty) in
+      let ofs := align ofs (CapAST.typesize ty) in
       One(S Outgoing ofs ty)
-      :: rec ri rf (ofs + (if Archi.ptr64 then 2 else typesize ty))
+      :: rec ri rf (ofs + (if Archi.ptr64 then 2 else CapAST.typesize ty))
   end.
 
-Definition float_arg (va: bool) (ri rf ofs: Z) (ty: typ)
-                     (rec: Z -> Z -> Z -> list (rpair loc)) :=
+Definition float_arg (va: bool) (ri rf ofs: Z) (ty: captyp)
+                     (rec: Z -> Z -> Z -> list (rpair caploc)) :=
   match list_nth_z (if va then nil else float_param_regs) rf with
   | Some r =>
       One (R r) :: rec ri (rf + 1) ofs
@@ -240,62 +244,63 @@ Definition float_arg (va: bool) (ri rf ofs: Z) (ty: typ)
          so try to put the argument in an extra FP register while
          reserving an integer register or register pair into which
          fixup code will move the extra FP register. *)
-      let regpair := negb Archi.ptr64 && zeq (typesize ty) 2 in
+      let regpair := negb Archi.ptr64 && zeq (CapAST.typesize ty) 2 in
       let ri' := if va && regpair then align ri 2 else ri in
       match list_nth_z float_extra_param_regs ri' with
       | Some r =>
-          let ri'' := ri' + (if Archi.ptr64 then 1 else typesize ty) in
+          let ri'' := ri' + (if Archi.ptr64 then 1 else CapAST.typesize ty) in
           let ofs'' := if regpair && zeq ri' 7 then ofs + 1 else ofs in
           One (R r) :: rec ri'' rf ofs''
       | None =>
           (* We are out of integer registers, pass argument on stack *)
-            let ofs := align ofs (typesize ty) in
+            let ofs := align ofs (CapAST.typesize ty) in
             One(S Outgoing ofs ty)
-            :: rec ri' rf (ofs + (if Archi.ptr64 then 2 else typesize ty))
+            :: rec ri' rf (ofs + (if Archi.ptr64 then 2 else CapAST.typesize ty))
       end
   end.
 
 Definition split_long_arg (va: bool) (ri rf ofs: Z)
-                          (rec: Z -> Z -> Z -> list (rpair loc)) :=
+                          (rec: Z -> Z -> Z -> list (rpair caploc)) :=
   let ri := if va then align ri 2 else ri in
   match list_nth_z int_param_regs ri, list_nth_z int_param_regs (ri + 1) with
   | Some r1, Some r2 =>
       Twolong (R r2) (R r1) :: rec (ri + 2) rf ofs
   | Some r1, None =>
-      Twolong (S Outgoing ofs Tint) (R r1) :: rec (ri + 1) rf (ofs + 1)
+      Twolong (S Outgoing ofs CTint) (R r1) :: rec (ri + 1) rf (ofs + 1)
   | None, _ =>
       let ofs := align ofs 2 in
-      Twolong (S Outgoing (ofs + 1) Tint) (S Outgoing ofs Tint) ::
+      Twolong (S Outgoing (ofs + 1) CTint) (S Outgoing ofs CTint) ::
       rec ri rf (ofs + 2)
   end.
 
 Fixpoint loc_arguments_rec
-    (tyl: list typ) (fixed ri rf ofs: Z) {struct tyl} : list (rpair loc) :=
+    (tyl: list captyp) (fixed ri rf ofs: Z) {struct tyl} : list (rpair caploc) :=
   match tyl with
   | nil => nil
-  | (Tint | Tany32) as ty :: tys =>
+  | (CTint | CTany32) as ty :: tys =>
       (* pass in one integer register or on stack *)
       int_arg ri rf ofs ty (loc_arguments_rec tys (fixed - 1))
-  | Tsingle as ty :: tys =>
+  | CTsingle as ty :: tys =>
       (* pass in one FP register or on stack.
          If vararg, reserve 1 integer register. *)
       float_arg (zle fixed 0) ri rf ofs ty (loc_arguments_rec tys (fixed - 1))
-  | Tlong as ty :: tys =>
+  | CTlong as ty :: tys =>
       if Archi.ptr64 then
         (* pass in one integer register or on stack *)
         int_arg ri rf ofs ty (loc_arguments_rec tys (fixed - 1))
       else
         (* pass in register pair or on stack; align register pair if vararg *)
         split_long_arg (zle fixed 0) ri rf ofs(loc_arguments_rec tys (fixed - 1))
-  | (Tfloat | Tany64) as ty :: tys =>
+  | (CTfloat | CTany64) as ty :: tys =>
       (* pass in one FP register or on stack.
          If vararg, reserve 1 or 2 integer registers. *)
       float_arg (zle fixed 0) ri rf ofs ty (loc_arguments_rec tys (fixed - 1))
+  | _ => nil (* FIXME *)
   end.
 
 (** Number of fixed arguments for a function with signature [s]. *)
 
-Definition fixed_arguments (s: signature) : Z :=
+Definition fixed_arguments (s: capsignature) : Z :=
   match s.(sig_cc).(cc_vararg) with
   | Some n => n
   | None => list_length_z s.(sig_args)
@@ -304,20 +309,20 @@ Definition fixed_arguments (s: signature) : Z :=
 (** [loc_arguments s] returns the list of locations where to store arguments
   when calling a function with signature [s].  *)
 
-Definition loc_arguments (s: signature) : list (rpair loc) :=
+Definition loc_arguments (s: capsignature) : list (rpair caploc) :=
   loc_arguments_rec s.(sig_args) (fixed_arguments s) 0 0 0.
 
 (** Argument locations are either non-temporary registers or [Outgoing]
   stack slots at nonnegative offsets. *)
 
-Definition loc_argument_acceptable (l: loc) : Prop :=
+Definition loc_argument_acceptable (l: caploc) : Prop :=
   match l with
   | R r => is_callee_save r = false
   | S Outgoing ofs ty => ofs >= 0 /\ (typealign ty | ofs)
   | _ => False
   end.
 
-Definition loc_argument_acceptable_stronger (l: loc) : Prop :=
+Definition loc_argument_acceptable_stronger (l: caploc) : Prop :=
   match l with
   | R r => is_callee_save r = false /\ r <> R30
   | S Outgoing ofs ty => ofs >= 0 /\ (typealign ty | ofs)
@@ -325,204 +330,208 @@ Definition loc_argument_acceptable_stronger (l: loc) : Prop :=
   end.
 
 Lemma loc_argument_acceptable_stronger_loc_argument_acceptable:
-  forall (l: loc),
+  forall (l: caploc),
     loc_argument_acceptable_stronger l ->
     loc_argument_acceptable l.
 Proof.
   destruct l; simpl; intuition.
 Qed.
 
-Lemma loc_arguments_rec_charact_stronger:
-  forall va tyl ri rf ofs p,
-  ofs >= 0 ->
-  In p (loc_arguments_rec va tyl ri rf ofs) -> forall_rpair loc_argument_acceptable_stronger p.
-Proof.
-  set (OK := fun (l: list (rpair loc)) =>
-             forall p, In p l -> forall_rpair loc_argument_acceptable_stronger p).
-  set (OKF := fun (f: Z -> Z -> Z -> list (rpair loc)) =>
-              forall ri rf ofs, ofs >= 0 -> OK (f ri rf ofs)).
-  assert (CSI: forall r, In r int_param_regs -> is_callee_save r = false /\ r <> R30).
-  { decide_goal. }
-  assert (CSF: forall r, In r float_param_regs -> is_callee_save r = false /\ r <> R30).
-  { decide_goal. }
-  assert (CSFX: forall r, In r float_extra_param_regs -> is_callee_save r = false /\ r <> R30).
-  { decide_goal. }
-  assert (AL: forall ofs ty, ofs >= 0 -> align ofs (typesize ty) >= 0).
-  { intros. 
-    assert (ofs <= align ofs (typesize ty)) by (apply align_le; apply typesize_pos).
-    lia. }
-  assert (ALD: forall ofs ty, ofs >= 0 -> (typealign ty | align ofs (typesize ty))).
-  { intros. eapply Z.divide_trans. apply typealign_typesize.
-    apply align_divides. apply typesize_pos. }
-  assert (SK: (if Archi.ptr64 then 2 else 1) > 0).
-  { destruct Archi.ptr64; lia. }
-  assert (SKK: forall ty, (if Archi.ptr64 then 2 else typesize ty) > 0).
-  { intros. destruct Archi.ptr64. lia. apply typesize_pos.  }
-  assert (A: forall ri rf ofs ty f,
-             OKF f -> ofs >= 0 -> OK (int_arg ri rf ofs ty f)).
-  { intros until f; intros OF OO; red; unfold int_arg; intros.
-    destruct (list_nth_z int_param_regs ri) as [r|] eqn:NTH; destruct H.
-  - subst p; simpl. apply CSI. eapply list_nth_z_in; eauto. 
-  - eapply OF; eauto. 
-  - subst p; simpl. auto using align_divides, typealign_pos.
-  - eapply OF; [idtac|eauto].
-    generalize (AL ofs ty OO) (SKK ty); lia.
-  }
-  assert (B: forall va ri rf ofs ty f,
-             OKF f -> ofs >= 0 -> OK (float_arg va ri rf ofs ty f)).
-  { intros until f; intros OF OO; red; unfold float_arg; intros.
-    destruct (list_nth_z (if va then nil else float_param_regs) rf) as [r|] eqn:NTH.
-  - destruct H.
-    + subst p; simpl. apply CSF. destruct va. simpl in NTH; discriminate. eapply list_nth_z_in; eauto.
-    + eapply OF; eauto.
-  - set (regpair := negb Archi.ptr64 && zeq (typesize ty) 2) in *.
-    set (ri' := if va && regpair then align ri 2 else ri) in *.
-    destruct (list_nth_z float_extra_param_regs ri') as [r|] eqn:NTH'; destruct H.
-    + subst p; simpl. apply CSFX. eapply list_nth_z_in; eauto.
-    + eapply OF; [|eauto]. destruct (regpair && zeq ri' 7); lia.
-    + subst p; simpl. auto.
-    + eapply OF; [|eauto]. generalize (AL ofs ty OO) (SKK ty); lia.
-  }
-  assert (C: forall va ri rf ofs f,
-             OKF f -> ofs >= 0 -> OK (split_long_arg va ri rf ofs f)).
-  { intros until f; intros OF OO; unfold split_long_arg.
-    set (ri' := if va then align ri 2 else ri).
-    set (ofs' := align ofs 2).
-    assert (OO': ofs' >= 0) by (apply (AL ofs Tlong); auto).
-    destruct (list_nth_z int_param_regs ri') as [r1|] eqn:NTH1;
-    [destruct (list_nth_z int_param_regs (ri'+1)) as [r2|] eqn:NTH2 | idtac].
-  - red; simpl; intros; destruct H.
-    + subst p; split; apply CSI; eauto using list_nth_z_in.
-    + eapply OF; [idtac|eauto]. lia.
-  - red; simpl; intros; destruct H.
-    + subst p; split. split; auto using Z.divide_1_l. apply CSI; eauto using list_nth_z_in.
-    + eapply OF; [idtac|eauto]. lia.
-  - red; simpl; intros; destruct H.
-    + subst p; repeat split; auto using Z.divide_1_l. lia. 
-    + eapply OF; [idtac|eauto]. lia.
-  }
-  cut (forall tyl fixed ri rf ofs, ofs >= 0 -> OK (loc_arguments_rec tyl fixed ri rf ofs)).
-  unfold OK. eauto.
-  induction tyl as [ | ty1 tyl]; intros until ofs; intros OO; simpl.
-- red; simpl; tauto.
-- destruct ty1.
-+ (* int *) apply A; unfold OKF; auto.
-+ (* float *) apply B; unfold OKF; auto.
-+ (* long *)
-  destruct Archi.ptr64.
-  apply A; unfold OKF; auto.
-  apply C; unfold OKF; auto.
-+ (* single *) apply B; unfold OKF; auto.
-+ (* any32 *) apply A; unfold OKF; auto.
-+ (* any64 *) apply B; unfold OKF; auto.
-Qed.
+(* FIXME *)
+(* Lemma loc_arguments_rec_charact_stronger: *)
+(*   forall va tyl ri rf ofs p, *)
+(*   ofs >= 0 -> *)
+(*   In p (loc_arguments_rec va tyl ri rf ofs) -> forall_rpair loc_argument_acceptable_stronger p. *)
+(* Proof. *)
+(*   set (OK := fun (l: list (rpair loc)) => *)
+(*              forall p, In p l -> forall_rpair loc_argument_acceptable_stronger p). *)
+(*   set (OKF := fun (f: Z -> Z -> Z -> list (rpair loc)) => *)
+(*               forall ri rf ofs, ofs >= 0 -> OK (f ri rf ofs)). *)
+(*   assert (CSI: forall r, In r int_param_regs -> is_callee_save r = false /\ r <> R30). *)
+(*   { decide_goal. } *)
+(*   assert (CSF: forall r, In r float_param_regs -> is_callee_save r = false /\ r <> R30). *)
+(*   { decide_goal. } *)
+(*   assert (CSFX: forall r, In r float_extra_param_regs -> is_callee_save r = false /\ r <> R30). *)
+(*   { decide_goal. } *)
+(*   assert (AL: forall ofs ty, ofs >= 0 -> align ofs (typesize ty) >= 0). *)
+(*   { intros.  *)
+(*     assert (ofs <= align ofs (typesize ty)) by (apply align_le; apply typesize_pos). *)
+(*     lia. } *)
+(*   assert (ALD: forall ofs ty, ofs >= 0 -> (typealign ty | align ofs (typesize ty))). *)
+(*   { intros. eapply Z.divide_trans. apply typealign_typesize. *)
+(*     apply align_divides. apply typesize_pos. } *)
+(*   assert (SK: (if Archi.ptr64 then 2 else 1) > 0). *)
+(*   { destruct Archi.ptr64; lia. } *)
+(*   assert (SKK: forall ty, (if Archi.ptr64 then 2 else typesize ty) > 0). *)
+(*   { intros. destruct Archi.ptr64. lia. apply typesize_pos.  } *)
+(*   assert (A: forall ri rf ofs ty f, *)
+(*              OKF f -> ofs >= 0 -> OK (int_arg ri rf ofs ty f)). *)
+(*   { intros until f; intros OF OO; red; unfold int_arg; intros. *)
+(*     destruct (list_nth_z int_param_regs ri) as [r|] eqn:NTH; destruct H. *)
+(*   - subst p; simpl. apply CSI. eapply list_nth_z_in; eauto.  *)
+(*   - eapply OF; eauto.  *)
+(*   - subst p; simpl. auto using align_divides, typealign_pos. *)
+(*   - eapply OF; [idtac|eauto]. *)
+(*     generalize (AL ofs ty OO) (SKK ty); lia. *)
+(*   } *)
+(*   assert (B: forall va ri rf ofs ty f, *)
+(*              OKF f -> ofs >= 0 -> OK (float_arg va ri rf ofs ty f)). *)
+(*   { intros until f; intros OF OO; red; unfold float_arg; intros. *)
+(*     destruct (list_nth_z (if va then nil else float_param_regs) rf) as [r|] eqn:NTH. *)
+(*   - destruct H. *)
+(*     + subst p; simpl. apply CSF. destruct va. simpl in NTH; discriminate. eapply list_nth_z_in; eauto. *)
+(*     + eapply OF; eauto. *)
+(*   - set (regpair := negb Archi.ptr64 && zeq (typesize ty) 2) in *. *)
+(*     set (ri' := if va && regpair then align ri 2 else ri) in *. *)
+(*     destruct (list_nth_z float_extra_param_regs ri') as [r|] eqn:NTH'; destruct H. *)
+(*     + subst p; simpl. apply CSFX. eapply list_nth_z_in; eauto. *)
+(*     + eapply OF; [|eauto]. destruct (regpair && zeq ri' 7); lia. *)
+(*     + subst p; simpl. auto. *)
+(*     + eapply OF; [|eauto]. generalize (AL ofs ty OO) (SKK ty); lia. *)
+(*   } *)
+(*   assert (C: forall va ri rf ofs f, *)
+(*              OKF f -> ofs >= 0 -> OK (split_long_arg va ri rf ofs f)). *)
+(*   { intros until f; intros OF OO; unfold split_long_arg. *)
+(*     set (ri' := if va then align ri 2 else ri). *)
+(*     set (ofs' := align ofs 2). *)
+(*     assert (OO': ofs' >= 0) by (apply (AL ofs Tlong); auto). *)
+(*     destruct (list_nth_z int_param_regs ri') as [r1|] eqn:NTH1; *)
+(*     [destruct (list_nth_z int_param_regs (ri'+1)) as [r2|] eqn:NTH2 | idtac]. *)
+(*   - red; simpl; intros; destruct H. *)
+(*     + subst p; split; apply CSI; eauto using list_nth_z_in. *)
+(*     + eapply OF; [idtac|eauto]. lia. *)
+(*   - red; simpl; intros; destruct H. *)
+(*     + subst p; split. split; auto using Z.divide_1_l. apply CSI; eauto using list_nth_z_in. *)
+(*     + eapply OF; [idtac|eauto]. lia. *)
+(*   - red; simpl; intros; destruct H. *)
+(*     + subst p; repeat split; auto using Z.divide_1_l. lia.  *)
+(*     + eapply OF; [idtac|eauto]. lia. *)
+(*   } *)
+(*   cut (forall tyl fixed ri rf ofs, ofs >= 0 -> OK (loc_arguments_rec tyl fixed ri rf ofs)). *)
+(*   unfold OK. eauto. *)
+(*   induction tyl as [ | ty1 tyl]; intros until ofs; intros OO; simpl. *)
+(* - red; simpl; tauto. *)
+(* - destruct ty1. *)
+(* + (* int *) apply A; unfold OKF; auto. *)
+(* + (* float *) apply B; unfold OKF; auto. *)
+(* + (* long *) *)
+(*   destruct Archi.ptr64. *)
+(*   apply A; unfold OKF; auto. *)
+(*   apply C; unfold OKF; auto. *)
+(* + (* single *) apply B; unfold OKF; auto. *)
+(* + (* any32 *) apply A; unfold OKF; auto. *)
+(* + (* any64 *) apply B; unfold OKF; auto. *)
+(* Qed. *)
 
 (* Alternative proof based on stronger version:
   intros. eapply loc_arguments_rec_charact_stronger in H0; auto.
   destruct p; simpl in *; intuition; auto using loc_argument_acceptable_stronger_loc_argument_acceptable.
  *)
-Lemma loc_arguments_rec_charact:
-  forall va tyl ri rf ofs p,
-  ofs >= 0 ->
-  In p (loc_arguments_rec va tyl ri rf ofs) -> forall_rpair loc_argument_acceptable p.
-Proof.
-  set (OK := fun (l: list (rpair loc)) =>
-             forall p, In p l -> forall_rpair loc_argument_acceptable p).
-  set (OKF := fun (f: Z -> Z -> Z -> list (rpair loc)) =>
-              forall ri rf ofs, ofs >= 0 -> OK (f ri rf ofs)).
-  assert (CSI: forall r, In r int_param_regs -> is_callee_save r = false).
-  { decide_goal. }
-  assert (CSF: forall r, In r float_param_regs -> is_callee_save r = false).
-  { decide_goal. }
-  assert (CSFX: forall r, In r float_extra_param_regs -> is_callee_save r = false).
-  { decide_goal. }
-  assert (AL: forall ofs ty, ofs >= 0 -> align ofs (typesize ty) >= 0).
-  { intros. 
-    assert (ofs <= align ofs (typesize ty)) by (apply align_le; apply typesize_pos).
-    lia. }
-  assert (ALD: forall ofs ty, ofs >= 0 -> (typealign ty | align ofs (typesize ty))).
-  { intros. eapply Z.divide_trans. apply typealign_typesize.
-    apply align_divides. apply typesize_pos. }
-  assert (SK: (if Archi.ptr64 then 2 else 1) > 0).
-  { destruct Archi.ptr64; lia. }
-  assert (SKK: forall ty, (if Archi.ptr64 then 2 else typesize ty) > 0).
-  { intros. destruct Archi.ptr64. lia. apply typesize_pos.  }
-  assert (A: forall ri rf ofs ty f,
-             OKF f -> ofs >= 0 -> OK (int_arg ri rf ofs ty f)).
-  { intros until f; intros OF OO; red; unfold int_arg; intros.
-    destruct (list_nth_z int_param_regs ri) as [r|] eqn:NTH; destruct H.
-  - subst p; simpl. apply CSI. eapply list_nth_z_in; eauto. 
-  - eapply OF; eauto. 
-  - subst p; simpl. auto using align_divides, typealign_pos.
-  - eapply OF; [idtac|eauto].
-    generalize (AL ofs ty OO) (SKK ty); lia.
-  }
-  assert (B: forall va ri rf ofs ty f,
-             OKF f -> ofs >= 0 -> OK (float_arg va ri rf ofs ty f)).
-  { intros until f; intros OF OO; red; unfold float_arg; intros.
-    destruct (list_nth_z (if va then nil else float_param_regs) rf) as [r|] eqn:NTH.
-  - destruct H.
-    + subst p; simpl. apply CSF. destruct va. simpl in NTH; discriminate. eapply list_nth_z_in; eauto.
-    + eapply OF; eauto.
-  - set (regpair := negb Archi.ptr64 && zeq (typesize ty) 2) in *.
-    set (ri' := if va && regpair then align ri 2 else ri) in *.
-    destruct (list_nth_z float_extra_param_regs ri') as [r|] eqn:NTH'; destruct H.
-    + subst p; simpl. apply CSFX. eapply list_nth_z_in; eauto.
-    + eapply OF; [|eauto]. destruct (regpair && zeq ri' 7); lia.
-    + subst p; simpl. auto.
-    + eapply OF; [|eauto]. generalize (AL ofs ty OO) (SKK ty); lia.
-  }
-  assert (C: forall va ri rf ofs f,
-             OKF f -> ofs >= 0 -> OK (split_long_arg va ri rf ofs f)).
-  { intros until f; intros OF OO; unfold split_long_arg.
-    set (ri' := if va then align ri 2 else ri).
-    set (ofs' := align ofs 2).
-    assert (OO': ofs' >= 0) by (apply (AL ofs Tlong); auto).
-    destruct (list_nth_z int_param_regs ri') as [r1|] eqn:NTH1;
-    [destruct (list_nth_z int_param_regs (ri'+1)) as [r2|] eqn:NTH2 | idtac].
-  - red; simpl; intros; destruct H.
-    + subst p; split; apply CSI; eauto using list_nth_z_in.
-    + eapply OF; [idtac|eauto]. lia.
-  - red; simpl; intros; destruct H.
-    + subst p; split. split; auto using Z.divide_1_l. apply CSI; eauto using list_nth_z_in.
-    + eapply OF; [idtac|eauto]. lia.
-  - red; simpl; intros; destruct H.
-    + subst p; repeat split; auto using Z.divide_1_l. lia. 
-    + eapply OF; [idtac|eauto]. lia.
-  }
-  cut (forall tyl fixed ri rf ofs, ofs >= 0 -> OK (loc_arguments_rec tyl fixed ri rf ofs)).
-  unfold OK. eauto.
-  induction tyl as [ | ty1 tyl]; intros until ofs; intros OO; simpl.
-- red; simpl; tauto.
-- destruct ty1.
-+ (* int *) apply A; unfold OKF; auto.
-+ (* float *) apply B; unfold OKF; auto.
-+ (* long *)
-  destruct Archi.ptr64.
-  apply A; unfold OKF; auto.
-  apply C; unfold OKF; auto.
-+ (* single *) apply B; unfold OKF; auto.
-+ (* any32 *) apply A; unfold OKF; auto.
-+ (* any64 *) apply B; unfold OKF; auto.
-Qed.
+(* FIXME *)
+(* Lemma loc_arguments_rec_charact: *)
+(*   forall va tyl ri rf ofs p, *)
+(*   ofs >= 0 -> *)
+(*   In p (loc_arguments_rec va tyl ri rf ofs) -> forall_rpair loc_argument_acceptable p. *)
+(* Proof. *)
+(*   set (OK := fun (l: list (rpair loc)) => *)
+(*              forall p, In p l -> forall_rpair loc_argument_acceptable p). *)
+(*   set (OKF := fun (f: Z -> Z -> Z -> list (rpair loc)) => *)
+(*               forall ri rf ofs, ofs >= 0 -> OK (f ri rf ofs)). *)
+(*   assert (CSI: forall r, In r int_param_regs -> is_callee_save r = false). *)
+(*   { decide_goal. } *)
+(*   assert (CSF: forall r, In r float_param_regs -> is_callee_save r = false). *)
+(*   { decide_goal. } *)
+(*   assert (CSFX: forall r, In r float_extra_param_regs -> is_callee_save r = false). *)
+(*   { decide_goal. } *)
+(*   assert (AL: forall ofs ty, ofs >= 0 -> align ofs (typesize ty) >= 0). *)
+(*   { intros.  *)
+(*     assert (ofs <= align ofs (typesize ty)) by (apply align_le; apply typesize_pos). *)
+(*     lia. } *)
+(*   assert (ALD: forall ofs ty, ofs >= 0 -> (typealign ty | align ofs (typesize ty))). *)
+(*   { intros. eapply Z.divide_trans. apply typealign_typesize. *)
+(*     apply align_divides. apply typesize_pos. } *)
+(*   assert (SK: (if Archi.ptr64 then 2 else 1) > 0). *)
+(*   { destruct Archi.ptr64; lia. } *)
+(*   assert (SKK: forall ty, (if Archi.ptr64 then 2 else typesize ty) > 0). *)
+(*   { intros. destruct Archi.ptr64. lia. apply typesize_pos.  } *)
+(*   assert (A: forall ri rf ofs ty f, *)
+(*              OKF f -> ofs >= 0 -> OK (int_arg ri rf ofs ty f)). *)
+(*   { intros until f; intros OF OO; red; unfold int_arg; intros. *)
+(*     destruct (list_nth_z int_param_regs ri) as [r|] eqn:NTH; destruct H. *)
+(*   - subst p; simpl. apply CSI. eapply list_nth_z_in; eauto.  *)
+(*   - eapply OF; eauto.  *)
+(*   - subst p; simpl. auto using align_divides, typealign_pos. *)
+(*   - eapply OF; [idtac|eauto]. *)
+(*     generalize (AL ofs ty OO) (SKK ty); lia. *)
+(*   } *)
+(*   assert (B: forall va ri rf ofs ty f, *)
+(*              OKF f -> ofs >= 0 -> OK (float_arg va ri rf ofs ty f)). *)
+(*   { intros until f; intros OF OO; red; unfold float_arg; intros. *)
+(*     destruct (list_nth_z (if va then nil else float_param_regs) rf) as [r|] eqn:NTH. *)
+(*   - destruct H. *)
+(*     + subst p; simpl. apply CSF. destruct va. simpl in NTH; discriminate. eapply list_nth_z_in; eauto. *)
+(*     + eapply OF; eauto. *)
+(*   - set (regpair := negb Archi.ptr64 && zeq (typesize ty) 2) in *. *)
+(*     set (ri' := if va && regpair then align ri 2 else ri) in *. *)
+(*     destruct (list_nth_z float_extra_param_regs ri') as [r|] eqn:NTH'; destruct H. *)
+(*     + subst p; simpl. apply CSFX. eapply list_nth_z_in; eauto. *)
+(*     + eapply OF; [|eauto]. destruct (regpair && zeq ri' 7); lia. *)
+(*     + subst p; simpl. auto. *)
+(*     + eapply OF; [|eauto]. generalize (AL ofs ty OO) (SKK ty); lia. *)
+(*   } *)
+(*   assert (C: forall va ri rf ofs f, *)
+(*              OKF f -> ofs >= 0 -> OK (split_long_arg va ri rf ofs f)). *)
+(*   { intros until f; intros OF OO; unfold split_long_arg. *)
+(*     set (ri' := if va then align ri 2 else ri). *)
+(*     set (ofs' := align ofs 2). *)
+(*     assert (OO': ofs' >= 0) by (apply (AL ofs Tlong); auto). *)
+(*     destruct (list_nth_z int_param_regs ri') as [r1|] eqn:NTH1; *)
+(*     [destruct (list_nth_z int_param_regs (ri'+1)) as [r2|] eqn:NTH2 | idtac]. *)
+(*   - red; simpl; intros; destruct H. *)
+(*     + subst p; split; apply CSI; eauto using list_nth_z_in. *)
+(*     + eapply OF; [idtac|eauto]. lia. *)
+(*   - red; simpl; intros; destruct H. *)
+(*     + subst p; split. split; auto using Z.divide_1_l. apply CSI; eauto using list_nth_z_in. *)
+(*     + eapply OF; [idtac|eauto]. lia. *)
+(*   - red; simpl; intros; destruct H. *)
+(*     + subst p; repeat split; auto using Z.divide_1_l. lia.  *)
+(*     + eapply OF; [idtac|eauto]. lia. *)
+(*   } *)
+(*   cut (forall tyl fixed ri rf ofs, ofs >= 0 -> OK (loc_arguments_rec tyl fixed ri rf ofs)). *)
+(*   unfold OK. eauto. *)
+(*   induction tyl as [ | ty1 tyl]; intros until ofs; intros OO; simpl. *)
+(* - red; simpl; tauto. *)
+(* - destruct ty1. *)
+(* + (* int *) apply A; unfold OKF; auto. *)
+(* + (* float *) apply B; unfold OKF; auto. *)
+(* + (* long *) *)
+(*   destruct Archi.ptr64. *)
+(*   apply A; unfold OKF; auto. *)
+(*   apply C; unfold OKF; auto. *)
+(* + (* single *) apply B; unfold OKF; auto. *)
+(* + (* any32 *) apply A; unfold OKF; auto. *)
+(* + (* any64 *) apply B; unfold OKF; auto. *)
+(* Qed. *)
 
-Lemma loc_arguments_acceptable_stronger:
-  forall (s: signature) (p: rpair loc),
-  In p (loc_arguments s) -> forall_rpair loc_argument_acceptable_stronger p.
-Proof.
-  unfold loc_arguments; intros. eapply loc_arguments_rec_charact_stronger; eauto. lia.
-Qed.
+(* FIXME *)
+(* Lemma loc_arguments_acceptable_stronger: *)
+(*   forall (s: capsignature) (p: rpair caploc), *)
+(*   In p (loc_arguments s) -> forall_rpair loc_argument_acceptable_stronger p. *)
+(* Proof. *)
+(*   unfold loc_arguments; intros. eapply loc_arguments_rec_charact_stronger; eauto. lia. *)
+(* Qed. *)
 
-Lemma loc_arguments_acceptable:
-  forall (s: signature) (p: rpair loc),
-  In p (loc_arguments s) -> forall_rpair loc_argument_acceptable p.
-Proof.
-  unfold loc_arguments; intros. eapply loc_arguments_rec_charact; eauto. lia.
-Qed.
+(* FIXME *)
+(* Lemma loc_arguments_acceptable: *)
+(*   forall (s: capsignature) (p: rpair caploc), *)
+(*   In p (loc_arguments s) -> forall_rpair loc_argument_acceptable p. *)
+(* Proof. *)
+(*   unfold loc_arguments; intros. eapply loc_arguments_rec_charact; eauto. lia. *)
+(* Qed. *)
 
 
 Lemma loc_arguments_main:
-  loc_arguments signature_main = nil.
+  loc_arguments capsignature_main = nil.
 Proof.
   reflexivity.
 Qed.
