cheririscV/CapMachregs.v
@@ -85,17 +85,17 @@ Instance Finite_mreg : Finite mreg := {
   Finite_elements_spec := all_mregs_complete
 }.
 
-Definition mreg_type (r: mreg): typ :=
+Definition mreg_type (r: mreg): captyp :=
   match r with
         | R5  | R6  | R7  | R8  | R9  | R10 | R11
   | R12 | R13 | R14 | R15 | R16 | R17 | R18 | R19
   | R20 | R21 | R22 | R23 | R24 | R25 | R26 | R27
-  | R28 | R29 | R30 => if Archi.ptr64 then Tany64 else Tany32
+  | R28 | R29 | R30 => if Archi.ptr64 then CTany64 else CTany32
 
   | F0  | F1  | F2  | F3  | F4  | F5  | F6  | F7
   | F8  | F9  | F10 | F11 | F12 | F13 | F14 | F15
   | F16 | F17 | F18 | F19 | F20 | F21 | F22 | F23
-  | F24 | F25 | F26 | F27 | F28 | F29 | F30 | F31 => Tany64
+  | F24 | F25 | F26 | F27 | F28 | F29 | F30 | F31 => CTany64
   end.
 
 Definition mreg_captype (r: mreg): captyp :=
