cheririscV/CapConventions.v
@@ -22,36 +22,37 @@ Require Export CapConventions1.
     [arch/abi/Conventions1.v].  This file adds various processor-independent
     definitions and lemmas. *)
 
-Lemma loc_arguments_acceptable_2:
-  forall s l,
-  In l (regs_of_rpairs (loc_arguments s)) -> loc_argument_acceptable l.
-Proof.
-  intros until l. generalize (loc_arguments_acceptable s). generalize (loc_arguments s).
-  induction l0 as [ | p pl]; simpl; intros.
-- contradiction.
-- rewrite in_app_iff in H0. destruct H0.
-  exploit H; eauto. destruct p; simpl in *; intuition congruence.
-  apply IHpl; auto.
-Qed.
+(* FIXME *)
+(* Lemma loc_arguments_acceptable_2: *)
+(*   forall s l, *)
+(*   In l (regs_of_rpairs (loc_arguments s)) -> loc_argument_acceptable l. *)
+(* Proof. *)
+(*   intros until l. generalize (loc_arguments_acceptable s). generalize (loc_arguments s). *)
+(*   induction l0 as [ | p pl]; simpl; intros. *)
+(* - contradiction. *)
+(* - rewrite in_app_iff in H0. destruct H0. *)
+(*   exploit H; eauto. destruct p; simpl in *; intuition congruence. *)
+(*   apply IHpl; auto. *)
+(* Qed. *)
 
 (** ** Stack size of function arguments *)
 
 (** [size_arguments s] returns the number of [Outgoing] slots used
   to call a function with signature [s]. *)
 
-Definition max_outgoing_1 (accu: Z) (l: loc) : Z :=
+Definition max_outgoing_1 (accu: Z) (l: caploc) : Z :=
   match l with
-  | S Outgoing ofs ty => Z.max accu (ofs + typesize ty)
+  | S Outgoing ofs ty => Z.max accu (ofs + CapAST.typesize ty)
   | _ => accu
   end.
 
-Definition max_outgoing_2 (accu: Z) (rl: rpair loc) : Z :=
+Definition max_outgoing_2 (accu: Z) (rl: rpair caploc) : Z :=
   match rl with
   | One l => max_outgoing_1 accu l
   | Twolong l1 l2 => max_outgoing_1 (max_outgoing_1 accu l1) l2
   end.
 
-Definition size_arguments (s: signature) : Z :=
+Definition size_arguments (s: capsignature) : Z :=
   List.fold_left max_outgoing_2 (loc_arguments s) 0.
 
 (** The offsets of [Outgoing] arguments are below [size_arguments s]. *)
@@ -73,33 +74,34 @@ Proof.
   intros. apply fold_max_outgoing_above.
 Qed.
 
-Lemma loc_arguments_bounded:
-  forall (s: signature) (ofs: Z) (ty: typ),
-  In (S Outgoing ofs ty) (regs_of_rpairs (loc_arguments s)) ->
-  ofs + typesize ty <= size_arguments s.
-Proof.
-  intros until ty.
-  assert (A: forall n l, n <= max_outgoing_1 n l).
-  { intros; unfold max_outgoing_1. destruct l as [_ | []]; extlia. }
-  assert (B: forall p n,
-             In (S Outgoing ofs ty) (regs_of_rpair p) ->
-             ofs + typesize ty <= max_outgoing_2 n p).
-  { intros. destruct p; simpl in H; intuition; subst; simpl.
-  - extlia.
-  - eapply Z.le_trans. 2: apply A. extlia.
-  - extlia. }
-  assert (C: forall l n,
-             In (S Outgoing ofs ty) (regs_of_rpairs l) ->
-             ofs + typesize ty <= fold_left max_outgoing_2 l n).
-  { induction l; simpl; intros.
-  - contradiction.
-  - rewrite in_app_iff in H. destruct H.
-  + eapply Z.le_trans. eapply B; eauto.
-    apply Z.ge_le. apply fold_max_outgoing_above.
-  + apply IHl; auto.
-  }
-  apply C. 
-Qed.
+(* FIXME *)
+(* Lemma loc_arguments_bounded: *)
+(*   forall (s: capsignature) (ofs: Z) (ty: captyp), *)
+(*   In (S Outgoing ofs ty) (regs_of_rpairs (loc_arguments s)) -> *)
+(*   ofs + CapAST.typesize ty <= size_arguments s. *)
+(* Proof. *)
+(*   intros until ty. *)
+(*   assert (A: forall n l, n <= max_outgoing_1 n l). *)
+(*   { intros; unfold max_outgoing_1. destruct l as [_ | []]; extlia. } *)
+(*   assert (B: forall p n, *)
+(*              In (S Outgoing ofs ty) (regs_of_rpair p) -> *)
+(*              ofs + typesize ty <= max_outgoing_2 n p). *)
+(*   { intros. destruct p; simpl in H; intuition; subst; simpl. *)
+(*   - extlia. *)
+(*   - eapply Z.le_trans. 2: apply A. extlia. *)
+(*   - extlia. } *)
+(*   assert (C: forall l n, *)
+(*              In (S Outgoing ofs ty) (regs_of_rpairs l) -> *)
+(*              ofs + typesize ty <= fold_left max_outgoing_2 l n). *)
+(*   { induction l; simpl; intros. *)
+(*   - contradiction. *)
+(*   - rewrite in_app_iff in H. destruct H. *)
+(*   + eapply Z.le_trans. eapply B; eauto. *)
+(*     apply Z.ge_le. apply fold_max_outgoing_above. *)
+(*   + apply IHl; auto. *)
+(*   } *)
+(*   apply C.  *)
+(* Qed. *)
 
 (** ** Location of function parameters *)
 
@@ -108,45 +110,46 @@ Qed.
   viewed as [Outgoing] slots by the caller, are accessed via [Incoming]
   slots (at the same offsets and types) in the callee. *)
 
-Definition parameter_of_argument (l: loc) : loc :=
+Definition parameter_of_argument (l: caploc) : caploc :=
   match l with
   | S Outgoing n ty => S Incoming n ty
   | _ => l
   end.
 
-Definition loc_parameters (s: signature) : list (rpair loc) :=
+Definition loc_parameters (s: capsignature) : list (rpair caploc) :=
   List.map (map_rpair parameter_of_argument) (loc_arguments s).
 
-Lemma incoming_slot_in_parameters:
-  forall ofs ty sg,
-  In (S Incoming ofs ty) (regs_of_rpairs (loc_parameters sg)) ->
-  In (S Outgoing ofs ty) (regs_of_rpairs (loc_arguments sg)).
-Proof.
-  intros.
-  replace (regs_of_rpairs (loc_parameters sg)) with (List.map parameter_of_argument (regs_of_rpairs (loc_arguments sg))) in H.
-  change (S Incoming ofs ty) with (parameter_of_argument (S Outgoing ofs ty)) in H.
-  exploit list_in_map_inv. eexact H. intros [x [A B]]. simpl in A.
-  exploit loc_arguments_acceptable_2; eauto. unfold loc_argument_acceptable; intros.
-  destruct x; simpl in A; try discriminate.
-  destruct sl; try contradiction.
-  inv A. auto.
-  unfold loc_parameters. generalize (loc_arguments sg). induction l as [ | p l]; simpl; intros.
-  auto.
-  rewrite map_app. f_equal; auto. destruct p; auto.
-Qed.
+(* FIXME *)
+(* Lemma incoming_slot_in_parameters: *)
+(*   forall ofs ty sg, *)
+(*   In (S Incoming ofs ty) (regs_of_rpairs (loc_parameters sg)) -> *)
+(*   In (S Outgoing ofs ty) (regs_of_rpairs (loc_arguments sg)). *)
+(* Proof. *)
+(*   intros. *)
+(*   replace (regs_of_rpairs (loc_parameters sg)) with (List.map parameter_of_argument (regs_of_rpairs (loc_arguments sg))) in H. *)
+(*   change (S Incoming ofs ty) with (parameter_of_argument (S Outgoing ofs ty)) in H. *)
+(*   exploit list_in_map_inv. eexact H. intros [x [A B]]. simpl in A. *)
+(*   exploit loc_arguments_acceptable_2; eauto. unfold loc_argument_acceptable; intros. *)
+(*   destruct x; simpl in A; try discriminate. *)
+(*   destruct sl; try contradiction. *)
+(*   inv A. auto. *)
+(*   unfold loc_parameters. generalize (loc_arguments sg). induction l as [ | p l]; simpl; intros. *)
+(*   auto. *)
+(*   rewrite map_app. f_equal; auto. destruct p; auto. *)
+(* Qed. *)
 
 (** * Tail calls *)
 
 (** A tail-call is possible for a signature if the corresponding
     arguments are all passed in registers. *)
 
-Definition tailcall_possible (s: signature) : Prop :=
+Definition tailcall_possible (s: capsignature) : Prop :=
   forall l, In l (regs_of_rpairs (loc_arguments s)) ->
   match l with R _ => True | S _ _ _ => False end.
 
 (** Decide whether a tailcall is possible. *)
 
-Definition tailcall_is_possible (sg: signature) : bool :=
+Definition tailcall_is_possible (sg: capsignature) : bool :=
   List.forallb
     (fun l => match l with R _ => true | S _ _ _ => false end)
     (regs_of_rpairs (loc_arguments sg)).
@@ -158,15 +161,16 @@ Proof.
   red; intros. apply H in H0. destruct l; [auto|discriminate].
 Qed.
 
-Lemma zero_size_arguments_tailcall_possible:
-  forall sg, size_arguments sg = 0 -> tailcall_possible sg.
-Proof.
-  intros; red; intros. exploit loc_arguments_acceptable_2; eauto.
-  unfold loc_argument_acceptable.
-  destruct l; intros. auto. destruct sl; try contradiction. destruct H1.
-  generalize (loc_arguments_bounded _ _ _ H0).
-  generalize (typesize_pos ty). lia.
-Qed.
+(* FIXME *)
+(* Lemma zero_size_arguments_tailcall_possible: *)
+(*   forall sg, size_arguments sg = 0 -> tailcall_possible sg. *)
+(* Proof. *)
+(*   intros; red; intros. exploit loc_arguments_acceptable_2; eauto. *)
+(*   unfold loc_argument_acceptable. *)
+(*   destruct l; intros. auto. destruct sl; try contradiction. destruct H1. *)
+(*   generalize (loc_arguments_bounded _ _ _ H0). *)
+(*   generalize (typesize_pos ty). lia. *)
+(* Qed. *)
 
 
 (** * Callee-save locations *)
@@ -186,7 +190,7 @@ are preserved across function calls, because they might not be preserved
 if the called function was compiled by another compiler. 
 *)
 
-Definition callee_save_loc (l: loc) :=
+Definition callee_save_loc (l: caploc) :=
   match l with
   | R r => is_callee_save r = true
   | S sl ofs ty => sl <> Outgoing
@@ -199,22 +203,24 @@ Definition agree_callee_save (ls1 ls2: Locmap.t) : Prop :=
 
 (** Useful lemmas to reason about the result of an external call. *)
 
-Lemma locmap_get_set_loc_result:
-  forall sg v rs l,
-  match l with R r => is_callee_save r = true | S _ _ _ => True end ->
-  Locmap.setpair (loc_result sg) v rs l = rs l.
-Proof.
-  intros. apply Locmap.gpo. 
-  assert (X: forall r, is_callee_save r = false -> Loc.diff l (R r)).
-  { intros. destruct l; simpl. congruence. auto. }
-  generalize (loc_result_caller_save sg). destruct (loc_result sg); simpl; intuition auto.
-Qed.
+(* FIXME *)
+(* Lemma locmap_get_set_loc_result: *)
+(*   forall sg v rs l, *)
+(*   match l with R r => is_callee_save r = true | S _ _ _ => True end -> *)
+(*   Locmap.setpair (loc_result sg) v rs l = rs l. *)
+(* Proof. *)
+(*   intros. apply Locmap.gpo.  *)
+(*   assert (X: forall r, is_callee_save r = false -> Loc.diff l (R r)). *)
+(*   { intros. destruct l; simpl. congruence. auto. } *)
+(*   generalize (loc_result_caller_save sg). destruct (loc_result sg); simpl; intuition auto. *)
+(* Qed. *)
 
-Lemma locmap_get_set_loc_result_callee_save:
-  forall sg v rs l,
-  callee_save_loc l ->
-  Locmap.setpair (loc_result sg) v rs l = rs l.
-Proof.
-  intros. apply locmap_get_set_loc_result. 
-  red in H; destruct l; auto.
-Qed.
+(* FIXME *)
+(* Lemma locmap_get_set_loc_result_callee_save: *)
+(*   forall sg v rs l, *)
+(*   callee_save_loc l -> *)
+(*   Locmap.setpair (loc_result sg) v rs l = rs l. *)
+(* Proof. *)
+(*   intros. apply locmap_get_set_loc_result.  *)
+(*   red in H; destruct l; auto. *)
+(* Qed. *)
