Makefile
@@ -148,7 +148,7 @@ SECURITY=RSC.v Split.v
 
 # Low-level backend (in cheririscV/)
 
-SECARCH=CapArchi.v CapAST.v OCapValues.v CapMemdata.v CapMemtype.v CapMemory.v CapGlobalenvs.v CapOp.v CapMachregs.v CapLocations.v CapAsm.v
+SECARCH=CapArchi.v CapAST.v OCapValues.v CapMemdata.v CapMemtype.v CapMemory.v CapGlobalenvs.v CapOp.v CapMachregs.v CapLocations.v CapAsm.v CapConventions1.v CapConventions.v
 
 # Parser
 
